# inspired by the discussion at https://github.com/w3c/dxwg/issues/1240

@prefix dtp:            <http://example.org/DataProduct/> .
@prefix rdf:            <http://www.w3.org/1999/02/22-rdf-syntax-ns#> .
@prefix rdfs:           <http://www.w3.org/2000/01/rdf-schema#> .
@prefix owl:            <http://www.w3.org/2002/07/owl#> .
@prefix sh:             <http://www.w3.org/ns/shacl#> .
@prefix xsd:            <http://www.w3.org/2001/XMLSchema#> .
@prefix skos:           <http://www.w3.org/2004/02/skos/core#> .
@prefix dct:            <http://purl.org/dc/terms/> .
@prefix dcat:           <http://www.w3.org/ns/dcat#> .
@prefix time:           <https://www.w3.org/TR/owl-time/#> .

dtp:DataProduct
    rdf:type            rdfs:Class ;
    rdfs:subClassOf     dcat:DataService ; 
    rdfs:label          "DataProduct"@en ;
    dct:description     "A data product consumes one or more datasets from its input port(s), performs computations, calculations, transformations on these input(s) and offers the resulting dataset(s) on its output port(s)."@en ;
    rdfs:comment        "A data product consumes one or more datasets from its input port(s), performs computations, calculations, transformations on these input(s) and offers the resulting dataset(s) on its output port(s)."@en ;
    skos:definition     "A data product consumes one or more datasets from its input port(s), performs computations, calculations, transformations on these input(s) and offers the resulting dataset(s) on its output port(s)."@en ;
.        

dtp:InputPort
    rdf:type            rdfs:Class ;
    rdfs:subClassOf     dcat:DataService ;
    rdfs:label          "InputPort"@en ;
    dct:description     "An input port of a data product is a data service that delivers a dataset into a data product using a specific delivery mechanism (file, API, database query, manual upload, stream, etc.)."@en ;
    rdfs:comment        "An input port of a data product is a data service that delivers a dataset into a data product using a specific delivery mechanism (file, API, database query, manual upload, stream, etc.)."@en ;
    skos:definition     "An input port of a data product is a data service that delivers a dataset into a data product using a specific delivery mechanism (file, API, database query, manual upload, stream, etc.)."@en ;
.

dtp:ApiInputPort
    rdf:type            rdfs:Class ;
    rdfs:subClassOf     dtp:InputPort ;
    rdfs:label          "ApiInputPort"@en ;
    dct:description     "An input port consuming data from an API call."@en ;
    rdfs:comment        "An input port consuming data from an API call."@en ;
    skos:definition     "An input port consuming data from an API call."@en ;
.

dtp:FileInputPort
    rdf:type            rdfs:Class ;
    rdfs:subClassOf     dtp:InputPort ;
    rdfs:label          "FileInputPort"@en ;
    dct:description     "An input port consuming data from a file."@en ;
    rdfs:comment        "An input port consuming data from a file."@en ;
    skos:definition     "An input port consuming data from a file."@en ;
.

dtp:OutputPort
    rdf:type            rdfs:Class ;
    rdfs:subClassOf     dcat:DataService ;
    rdfs:label          "OutputPort"@en ;
    dct:description     "An output port of a data product is a data service that delivers a dataset produced by the data product using a specific delivery mechanism (file, API, database query, manual download, stream, etc.)."@en ;
    rdfs:comment        "An output port of a data product is a data service that delivers a dataset produced by the data product using a specific delivery mechanism (file, API, database query, manual download, stream, etc.)."@en ;
    skos:definition     "An output port of a data product is a data service that delivers a dataset produced by the data product using a specific delivery mechanism (file, API, database query, manual download, stream, etc.)."@en ;
.

dtp:Dataset
    rdf:type            rdfs:Class ;
    rdfs:subClassOf     dcat:Dataset ;
    rdfs:label          "Dataset"@en ;
    dct:description     "A collection of data consumed by a data product on an input port, stored by a data product as internal representation, or offered by a data product on an output port."@en ;
    rdfs:comment        "A collection of data consumed by a data product on an input port, stored by a data product as internal representation, or offered by a data product on an output port."@en ;
    skos:definition     "A collection of data consumed by a data product on an input port, stored by a data product as internal representation, or offered by a data product on an output port."@en ;
.

dtp:hasInputPort
    rdf:type            rdfs:Property ;
    rdfs:domain         dtp:DataProduct ;
    rdfs:range          dtp:InputPort ;
    rdfs:label          "hasInputPort"@en ;
    dct:description     "An input port that a data product uses to consume data to produce an outcome."@en ;
    rdfs:comment        "An input port that a data product uses to consume data to produce an outcome."@en ;
    skos:definition     "An input port that a data product uses to consume data to produce an outcome."@en ;
.

dtp:hasOutputPort
    rdf:type            rdfs:Property ;
    rdfs:domain         dtp:DataProduct ;
    rdfs:range          dtp:OutputPort ;
    rdfs:label          "hasOutputPort"@en ;
    dct:description     "An output port that a data product uses to offer the dataset(s) it has produced."@en ;
    rdfs:comment        "An output port that a data product uses to offer the dataset(s) it has produced."@en ;
    skos:definition     "An output port that a data product uses to offer the dataset(s) it has produced."@en ;
.

dtp:hasDataModel
    rdf:type            rdfs:Property ;
    rdfs:domain         dtp:Dataset ;
    rdfs:range          rdfs:Resource ;
    rdfs:label          "hasDataModel"@en ;
    dct:description     "The IRI of the semantic model (a.k.a. context in linked data terms) describing structure, meaning and validation constraints of the dataset."@en ;
    rdfs:comment        "The IRI of the semantic model (a.k.a. context in linked data terms) describing structure, meaning and validation constraints of the dataset."@en ;
    skos:definition     "The IRI of the semantic model (a.k.a. context in linked data terms) describing structure, meaning and validation constraints of the dataset."@en ;
.

dtp:namePattern
    rdf:type            rdfs:Property ;
    rdfs:domain         dtp:FileInputPort ;
    rdfs:range          xsd:string ;
    rdfs:label          "namePattern"@en ;
    dct:description     "The regex pattern specifying the name of a resource, e.g. a file."@en ;
    rdfs:comment        "The regex pattern specifying the name of a resource, e.g. a file."@en ;
    skos:definition     "The regex pattern specifying the name of a resource, e.g. a file."@en ;
.

dtp:schedule
    rdf:type            rdfs:Property ;
    rdfs:domain         dtp:InputPort, dtp:OutputPort ;
    rdfs:range          time:GeneralDateTimeDescription ;
    rdfs:label          "schedule"@en ;
    dct:description     "The date/time description of the schedule of an activity (e.g. making an API call or polling for a file). If the datetime description is not pointing to an unambiguous, absolute point in time (e.g. a day of the week and a time, but no date, or just a specification of minutes or seconds) then the schedule is repeating, e.g. perform action every n hours/minutes/seconds or every day at the specific time."@en ;
    rdfs:comment        "The date/time description of the schedule of an activity (e.g. making an API call or polling for a file). If the datetime description is not pointing to an unambiguous, absolute point in time (e.g. a day of the week and a time, but no date, or just a specification of minutes or seconds) then the schedule is repeating, e.g. perform action every n hours/minutes/seconds or every day at the specific time."@en ;
    skos:definition     "The date/time description of the schedule of an activity (e.g. making an API call or polling for a file). If the datetime description is not pointing to an unambiguous, absolute point in time (e.g. a day of the week and a time, but no date, or just a specification of minutes or seconds) then the schedule is repeating, e.g. perform action every n hours/minutes/seconds or every day at the specific time."@en ;
.

dtp:format
    rdf:type            rdfs:Property ;
    rdfs:domain         dtp:InputPort, dtp:OutputPort ;
    rdfs:range          dtp:DataFormat ;
    rdfs:label          "format"@en ;
    dct:description     "The format of the data consumed resp. produced by an input/output port."@en ;
    rdfs:comment        "The format of the data consumed resp. produced by an input/output port."@en ;
    skos:definition     "The format of the data consumed resp. produced by an input/output port."@en ;
.

dtp:DataFormat
    rdf:type            rdfs:Class ;
    rdfs:label          "DataFormat"@en ;
    dct:description     "Describes the format of data, e.g. in a file or returned from an API call."@en ;
    rdfs:comment        "Describes the format of data, e.g. in a file or returned from an API call."@en ;
    skos:definition     "Describes the format of data, e.g. in a file or returned from an API call."@en ;
.

dtp:CSV
    rdf:type            dtp:DataFormat ;
    rdfs:label          "DataFormat"@en ;
    dct:description     "The CSV (comma-separated value) data format."@en ;
    rdfs:comment        "The CSV (comma-separated value) data format."@en ;
    skos:definition     "The CSV (comma-separated value) data format."@en ;
.

dtp:JSONLD
    rdf:type            dtp:DataFormat ;
    rdfs:label          "DataFormat"@en ;
    dct:description     "The JSON-LD (JSON linked data) format."@en ;
    rdfs:comment        "The JSON-LD (JSON linked data) format."@en ;
    skos:definition     "The JSON-LD (JSON linked data) format."@en ;
.

dtp:XML
    rdf:type            dtp:DataFormat ;
    rdfs:label          "DataFormat"@en ;
    dct:description     "The XML data format."@en ;
    rdfs:comment        "The XML data format."@en ;
    skos:definition     "The XML data format."@en ;
.

dtp:JSON
    rdf:type            dtp:DataFormat ;
    rdfs:label          "DataFormat"@en ;
    dct:description     "The JSON data format."@en ;
    rdfs:comment        "The JSON data format."@en ;
    skos:definition     "The JSON data format."@en ;
.

dtp:YAML
    rdf:type            dtp:DataFormat ;
    rdfs:label          "DataFormat"@en ;
    dct:description     "The YAML data format."@en ;
    rdfs:comment        "The YAML data format."@en ;
    skos:definition     "The YAML data format."@en ;
.

dtp:TURTLE
    rdf:type            dtp:DataFormat ;
    rdfs:label          "DataFormat"@en ;
    dct:description     "The Turtle serialization format."@en ;
    rdfs:comment        "The Turtle serialization format."@en ;
    skos:definition     "The Turtle serialization format."@en ;
.
